Refactoring is done.

hip/hip_graphmark_proofs.v
@@ -20,7 +20,7 @@ Require Import RamifyCoq.msl_application.GraphBi_Mark.
 Import RamifyCoq.msl_ext.seplog.OconNotation.
 
 Context {pSGG_Bi: pSpatialGraph_Graph_Bi}.
-Context {sSGG_Bi: sSpatialGraph_Graph_Bi}.
+Context {sSGG_Bi: sSpatialGraph_Graph_Bi bool unit}.
 Context {SGSA: SpatialGraphStrongAssum SGP}.
 
 Tactic Notation "LEM" constr(v) := (destruct (classic v); auto).
@@ -31,8 +31,8 @@ Module GraphMark <: Mgraphmark.
   Definition null_node : node := null.
   Definition valid : formula -> Prop := fun f => TT |-- f.
   Definition ptto_node : node -> bool -> node -> node -> formula := fun v d l r => vertex_at v (d, l, r).
-  Definition A : Type := Graph.
-  Definition graph : node -> A -> formula := fun x g => (@graph _ _ _ _ _ _ SGP _ x (GraphBi.Graph_SpatialGraph g)).
+  Definition A : Type := (@Graph _ bool unit).
+  Definition graph : node -> A -> formula := fun x g => (@graph _ _ _ _ _ _ SGP _ x (LGraph_SGraph (Graph_LGraph g))).
   Definition star : formula -> formula -> formula := sepcon.
   Definition and : formula -> formula -> formula := andp.
   Definition imp : formula -> formula -> formula := imp.
@@ -42,43 +42,47 @@ Module GraphMark <: Mgraphmark.
   Definition mwand : formula -> formula -> formula := ewand.
   Definition union : formula -> formula -> formula := ocon.
   Definition neq : bool -> bool -> formula := fun a b => prop (~ a = b).
-  Definition mark : A -> node -> A -> formula := fun g1 n g2 => prop (mark n g1 g2).
+  Definition mark : A -> node -> A -> formula := fun g1 n g2 => prop (mark n (Graph_LGraph g1) (Graph_LGraph g2)).
   Definition eq_notreach : A -> node -> A -> formula :=
-    fun g1 n g2 => prop ((unreachable_partial_spatialgraph (GraphBi.Graph_SpatialGraph g1) (n :: nil))
-                           -=- (unreachable_partial_spatialgraph (GraphBi.Graph_SpatialGraph g2) (n :: nil))).
-  Definition subset_reach : A -> node -> A -> formula := fun g1 n g2 => prop (Included (reachable g1 n) (reachable g2 n)).
+    fun g1 n g2 => prop ((unreachable_partial_spatialgraph (LGraph_SGraph (Graph_LGraph g1)) (n :: nil))
+                           -=- (unreachable_partial_spatialgraph (LGraph_SGraph (Graph_LGraph g2)) (n :: nil))).
+  Definition subset_reach : A -> node -> A -> formula := fun g1 n g2 => prop (Included (reachable (SGraph_PGraph (LGraph_SGraph (Graph_LGraph g1))) n)
+                                                                                       (reachable (SGraph_PGraph (LGraph_SGraph (Graph_LGraph g2))) n)).
   Definition lookup : A -> node -> bool -> node -> node -> formula :=
-    fun g x d l r => prop (vlabel g x = d /\ vvalid g x /\ vvalid g l /\ vvalid g r /\ dst g (x, L) = l /\ dst g (x, R) = r).
+    fun g x d l r => prop (vlabel (Graph_LGraph g) x = d /\ vvalid (SGraph_PGraph (LGraph_SGraph (Graph_LGraph g))) x /\
+                           vvalid (SGraph_PGraph (LGraph_SGraph (Graph_LGraph g))) l /\ vvalid (SGraph_PGraph (LGraph_SGraph (Graph_LGraph g))) r /\
+                           dst (SGraph_PGraph (LGraph_SGraph (Graph_LGraph g))) (x, L) = l /\ dst (SGraph_PGraph (LGraph_SGraph (Graph_LGraph g))) (x, R) = r).
   Definition update : A -> node -> bool -> node -> node -> A -> formula :=
-    fun g1 x d l r g2 => prop (exists (Hn : ~ is_null g1 x) (Hi : graph_gen.in_math g1 x l r), Graph_gen_update g1 x d l r Hi Hn = g2).
+    fun g1 x d l r g2 => prop (exists (Hn : ~ is_null (SGraph_PGraph (LGraph_SGraph (Graph_LGraph g1))) x)
+                                      (Hi : graph_gen.in_math (SGraph_PGraph (LGraph_SGraph (Graph_LGraph g1))) x l r), Graph_gen_update g1 x d l r Hi Hn = g2).
 
   Lemma update_is_mark1: forall (l r: addr) (G G1: A) x,
-      vvalid G x ->
-      dst G (x, L) = l -> dst G (x, R) = r ->
-      (exists (Hn : ~ is_null G x) (Hi : graph_gen.in_math G x l r),
+      vvalid (SGraph_PGraph (LGraph_SGraph (Graph_LGraph G))) x ->
+      dst (SGraph_PGraph (LGraph_SGraph (Graph_LGraph G))) (x, L) = l -> dst (SGraph_PGraph (LGraph_SGraph (Graph_LGraph G))) (x, R) = r ->
+      (exists (Hn : ~ is_null (SGraph_PGraph (LGraph_SGraph (Graph_LGraph G))) x) (Hi : graph_gen.in_math (SGraph_PGraph (LGraph_SGraph (Graph_LGraph G))) x l r),
           Graph_gen_update G x true l r Hi Hn = G1) ->
-      mark1 x G G1.
+      mark1 x (Graph_LGraph G) (Graph_LGraph G1).
   Proof.
     intros. unfold valid in H1. destruct H2 as [Hn [Hi ?]].
     rewrite <- H2. split; [|split]; simpl.
     + split; [|split; [|split]]; simpl; intros; auto.
       - unfold graph_gen.change_vvalid. intuition. subst; auto.
       - unfold graph_gen.change_evalid. intuition.
-        rewrite (@only_two_edges _ _ _ _ G _ _ (biGraph G)) in H4.
+        rewrite (@only_two_edges _ _ _ _ (SGraph_PGraph (LGraph_SGraph (Graph_LGraph G))) _ _ (biGraph G)) in H4.
         destruct H4; rewrite H3;
         [apply (@left_valid _ _ _ _ _ _ _ (biGraph G)) |
          apply (@right_valid _ _ _ _ _ _ _ (biGraph G))]; auto.
-      - unfold graph_gen.change_dst. destruct (equiv_dec (src G e) x); auto.
+      - unfold graph_gen.change_dst. destruct (equiv_dec (src (pg_lg (lg_gg G)) e) x); auto.
         unfold equiv in e0.
-        destruct (left_or_right G (biGraph G) x e e0); subst e; auto.
+        destruct (left_or_right (pg_lg (lg_gg G)) (biGraph G) x e e0); subst e; auto.
     + unfold graph_gen.update_vlabel. destruct (equiv_dec x x); intuition.
     + intros. unfold graph_gen.update_vlabel. destruct (equiv_dec x n'); intuition.
   Qed.
 
   Lemma marked_node_marked: forall (G1: A) (n: addr) (G2: A) (x: addr) (v: bool),
-      vlabel G1 x = true ->
-      WeakMarkGraph.mark n G1 G2 ->
-      vlabel G2 x = true.
+      vlabel (Graph_LGraph G1) x = true ->
+      WeakMarkGraph.mark n (Graph_LGraph G1) (Graph_LGraph G2) ->
+      vlabel (Graph_LGraph G2) x = true.
   Proof.
     intros. unfold WeakMarkGraph.mark. destruct H0 as [? ?]. specialize (H1 x).
     simpl in H1. symmetry. rewrite H1. left; auto.
@@ -92,31 +96,32 @@ Module GraphMark <: Mgraphmark.
   Proof.
     intros. unfold valid, imp, and, lookup, neq, mark, update.
     apply imp_andp_adjoint. normalize. destruct H as [? [? [? [? [? ?]]]]].
-    assert (mark1 x G G1) by (apply (update_is_mark1 l r); auto).
+    assert (mark1 x (Graph_LGraph G) (Graph_LGraph G1)) by (apply (update_is_mark1 l r); auto).
     apply andp_right; normalize.
     + destruct H0 as [Hn [Hi ?]].
       apply mark1_mark_list_mark with (r :: l :: nil); auto.
       - simpl. unfold Complement. unfold In. clear - H H1. subst v. intuition.
-      - apply gamma_step_list' with false; auto. simpl. unfold gamma.
+      - apply gamma_step_list' with false; auto. simpl.
         do 2 (f_equal; auto). subst v. apply Bool.not_true_is_false in H1. auto.
-      - hnf. apply (compond_intro (compond_relation Logic.eq (mark1 x)) _ _ G1 _).
-        apply (compond_intro Logic.eq (mark1 x) G G G1); auto.
+      - hnf. apply (compond_intro (compond_relation Logic.eq (mark1 x)) _ _ (Graph_LGraph G1) _).
+        apply (compond_intro Logic.eq (mark1 x) (Graph_LGraph G) (Graph_LGraph G) (Graph_LGraph G1)); auto.
         unfold mark_list. simpl. hnf.
         apply (compond_intro
-                 (compond_relation Logic.eq (Graph_Mark.mark r)) _ _ G2 _); auto.
-          apply (compond_intro Logic.eq (Graph_Mark.mark r) G1 G1 G2); auto.
+                 (compond_relation Logic.eq (Graph_Mark.mark r)) _ _ (Graph_LGraph G2) _); auto.
+          apply (compond_intro Logic.eq (Graph_Mark.mark r) (Graph_LGraph G1) (Graph_LGraph G1) (Graph_LGraph G2)); auto.
     + destruct H2, H3, H9. destruct H12 as [? ?]. split.
       - apply (marked_node_marked G2 l); auto. apply (marked_node_marked G1 r); auto. 
-      - assert (G ~=~ G3) by (transitivity G1; auto; transitivity G2; auto).
+      - assert ((SGraph_PGraph (LGraph_SGraph (Graph_LGraph G))) ~=~ (SGraph_PGraph (LGraph_SGraph (Graph_LGraph G3)))) by
+            (transitivity (SGraph_PGraph (LGraph_SGraph (Graph_LGraph G1))); auto; transitivity (SGraph_PGraph (LGraph_SGraph (Graph_LGraph G2))); auto).
         destruct H14 as [? [? [? ?]]]. split; [|split; [|split; [|split]]].
         * specialize (H14 x); intuition.
         * specialize (H14 l); intuition.
         * specialize (H14 r); intuition.
-        * assert (evalid G (x, L)) by
+        * assert (evalid (SGraph_PGraph (LGraph_SGraph (Graph_LGraph G))) (x, L)) by
               (apply (@left_valid _ _ _ _ _ _ _ (biGraph G)); auto).
           subst l. symmetry. specialize (H17 (x, L)).
           specialize (H15 (x, L)). intuition.
-        * assert (evalid G (x, R)) by
+        * assert (evalid (SGraph_PGraph (LGraph_SGraph (Graph_LGraph G))) (x, R)) by
               (apply (@right_valid _ _ _ _ _ _ _ (biGraph G)); auto).
           subst r. symmetry. specialize (H17 (x, R)).
           specialize (H15 (x, R)). intuition.
@@ -130,31 +135,32 @@ Module GraphMark <: Mgraphmark.
   Proof.
     intros. unfold valid, imp, and, lookup, neq, mark, update.
     apply imp_andp_adjoint. normalize. destruct H as [? [? [? [? [? ?]]]]].
-    assert (mark1 x G G1) by (apply (update_is_mark1 l r); auto).
+    assert (mark1 x (Graph_LGraph G) (Graph_LGraph G1)) by (apply (update_is_mark1 l r); auto).
     apply andp_right; normalize.
     + destruct H0 as [Hn [Hi ?]].
       apply mark1_mark_list_mark with (l :: r :: nil); auto.
       - simpl. unfold Complement. unfold In. clear - H H1. subst v. intuition.
-      - apply gamma_step_list with false; auto. simpl. unfold gamma.
+      - apply gamma_step_list with false; auto. simpl.
         do 2 (f_equal; auto). subst v. apply Bool.not_true_is_false in H1. auto.
-      - hnf. apply (compond_intro (compond_relation Logic.eq (mark1 x)) _ _ G1 _).
-        apply (compond_intro Logic.eq (mark1 x) G G G1); auto.
+      - hnf. apply (compond_intro (compond_relation Logic.eq (mark1 x)) _ _ (Graph_LGraph G1) _).
+        apply (compond_intro Logic.eq (mark1 x) (Graph_LGraph G) (Graph_LGraph G) (Graph_LGraph G1)); auto.
         unfold mark_list. simpl. hnf.
         apply (compond_intro
-                 (compond_relation Logic.eq (Graph_Mark.mark l)) _ _ G2 _); auto.
-          apply (compond_intro Logic.eq (Graph_Mark.mark l) G1 G1 G2); auto.
+                 (compond_relation Logic.eq (Graph_Mark.mark l)) _ _ (Graph_LGraph G2) _); auto.
+          apply (compond_intro Logic.eq (Graph_Mark.mark l) (Graph_LGraph G1) (Graph_LGraph G1) (Graph_LGraph G2)); auto.
     + destruct H2, H3, H9. destruct H12 as [? ?]. split.
       - apply (marked_node_marked G2 r); auto. apply (marked_node_marked G1 l); auto. 
-      - assert (G ~=~ G3) by (transitivity G1; auto; transitivity G2; auto).
+      - assert ((SGraph_PGraph (LGraph_SGraph (Graph_LGraph G))) ~=~ (SGraph_PGraph (LGraph_SGraph (Graph_LGraph G3)))) by
+            (transitivity (SGraph_PGraph (LGraph_SGraph (Graph_LGraph G1))); auto; transitivity (SGraph_PGraph (LGraph_SGraph (Graph_LGraph G2))); auto).
         destruct H14 as [? [? [? ?]]]. split; [|split; [|split; [|split]]].
         * specialize (H14 x); intuition.
         * specialize (H14 l); intuition.
         * specialize (H14 r); intuition.
-        * assert (evalid G (x, L)) by
+        * assert (evalid (SGraph_PGraph (LGraph_SGraph (Graph_LGraph G))) (x, L)) by
               (apply (@left_valid _ _ _ _ _ _ _ (biGraph G)); auto).
           subst l. symmetry. specialize (H17 (x, L)).
           specialize (H15 (x, L)). intuition.
-        * assert (evalid G (x, R)) by
+        * assert (evalid (SGraph_PGraph (LGraph_SGraph (Graph_LGraph G))) (x, R)) by
               (apply (@right_valid _ _ _ _ _ _ _ (biGraph G)); auto).
           subst r. symmetry. specialize (H17 (x, R)).
           specialize (H15 (x, R)). intuition.
@@ -177,10 +183,10 @@ Module GraphMark <: Mgraphmark.
       - apply partialgraph_proper; auto. unfold Complement. unfold In. hnf.
         split; intro z; unfold In; rewrite H6; auto.
       - destruct H7, H8. unfold Complement in *. unfold In in *.
-        unfold gamma. f_equal;[f_equal |]; [|apply dst_L_eq | apply dst_R_eq]; auto.
+        f_equal;[f_equal |]; [|apply dst_L_eq | apply dst_R_eq]; auto.
         destruct H. simpl in H11.
-        assert (~ reachable G x v0) by (intro; apply H9; rewrite reachable_through_set_single; auto).
-        destruct (Bool.bool_dec (vlabel G v0) true).
+        assert (~ reachable (SGraph_PGraph (LGraph_SGraph (Graph_LGraph G))) x v0) by (intro; apply H9; rewrite reachable_through_set_single; auto).
+        destruct (Bool.bool_dec (vlabel (Graph_LGraph G) v0) true).
         * rewrite e. apply H11. left; auto.
         * apply Bool.not_true_is_false in n. rewrite n. symmetry.
           apply Bool.not_true_is_false. intro. symmetry in H13. rewrite H11 in H13.
@@ -188,17 +194,17 @@ Module GraphMark <: Mgraphmark.
           apply reachable_by_is_reachable in H13. exfalso; auto.
     + unfold ext. destruct H as [[? ?] ?]. specialize (H6 y). simpl in H6.
       destruct H7 as [? [? [? ?]]].
-      LEM (G |= x ~o~> y satisfying (WeakMarkGraph.unmarked G)).
-      - assert (vlabel G1 y = true) by (symmetry; rewrite H6; right; auto).
+      LEM ((SGraph_PGraph (LGraph_SGraph (Graph_LGraph G))) |= x ~o~> y satisfying (WeakMarkGraph.unmarked (Graph_LGraph G))).
+      - assert (vlabel (Graph_LGraph G1) y = true) by (symmetry; rewrite H6; right; auto).
         apply (exp_right true). normalize. split; [|split;[|split;[|split; [|split]]]]; auto.
         * specialize (H7 y); intuition.
         * specialize (H7 l); intuition.
         * specialize (H7 r); intuition.
-        * assert (evalid G (y, L)) by
+        * assert (evalid (SGraph_PGraph (LGraph_SGraph (Graph_LGraph G))) (y, L)) by
               (apply (@left_valid _ _ _ _ _ _ _ (biGraph G)); auto).
           subst l. symmetry. specialize (H10 (y, L)).
           specialize (H8 (y, L)). intuition.
-        * assert (evalid G (y, R)) by
+        * assert (evalid (SGraph_PGraph (LGraph_SGraph (Graph_LGraph G))) (y, R)) by
               (apply (@right_valid _ _ _ _ _ _ _ (biGraph G)); auto).
           subst r. symmetry. specialize (H10 (y, R)).
           specialize (H8 (y, R)). intuition.
@@ -212,11 +218,11 @@ Module GraphMark <: Mgraphmark.
         * specialize (H7 y); intuition.
         * specialize (H7 l); intuition.
         * specialize (H7 r); intuition.
-        * assert (evalid G (y, L)) by
+        * assert (evalid (SGraph_PGraph (LGraph_SGraph (Graph_LGraph G))) (y, L)) by
               (apply (@left_valid _ _ _ _ _ _ _ (biGraph G)); auto).
           subst l. symmetry. specialize (H10 (y, L)).
           specialize (H8 (y, L)). intuition.
-        * assert (evalid G (y, R)) by
+        * assert (evalid (SGraph_PGraph (LGraph_SGraph (Graph_LGraph G))) (y, R)) by
               (apply (@right_valid _ _ _ _ _ _ _ (biGraph G)); auto).
           subst r. symmetry. specialize (H10 (y, R)).
           specialize (H8 (y, R)). intuition.
@@ -240,19 +246,21 @@ Module GraphMark <: Mgraphmark.
   Qed.
 
   Lemma lookup_graph_unfold: forall (G: A) x v l r,
-      vlabel G x = v -> vvalid G x -> vvalid G l -> vvalid G r -> dst G (x, L) = l ->
-      dst G (x, R) = r -> (graph x G = ptto_node x v l r ⊗ graph l G ⊗ graph r G).
+      vlabel (Graph_LGraph G) x = v -> vvalid (SGraph_PGraph (LGraph_SGraph (Graph_LGraph G))) x -> vvalid (SGraph_PGraph (LGraph_SGraph (Graph_LGraph G))) l ->
+      vvalid (SGraph_PGraph (LGraph_SGraph (Graph_LGraph G))) r -> dst (SGraph_PGraph (LGraph_SGraph (Graph_LGraph G))) (x, L) = l ->
+      dst (SGraph_PGraph (LGraph_SGraph (Graph_LGraph G))) (x, R) = r -> (graph x G = ptto_node x v l r ⊗ graph l G ⊗ graph r G).
   Proof.
     intros. unfold graph. unfold ptto_node. apply bi_graph_unfold; auto.
-    simpl. unfold gamma. f_equal; [f_equal|]; auto.
+    simpl. f_equal; [f_equal|]; auto.
   Qed.
 
   Lemma graph_graphs_eq_l:
-    forall (G: A) v x l r, vlabel G x = v -> vvalid G x -> vvalid G l -> vvalid G r ->
-                           dst G (x, L) = l -> dst G (x, R) = r ->
+    forall (G: A) v x l r, vlabel (Graph_LGraph G) x = v -> vvalid (SGraph_PGraph (LGraph_SGraph (Graph_LGraph G))) x ->
+                           vvalid (SGraph_PGraph (LGraph_SGraph (Graph_LGraph G))) l -> vvalid (SGraph_PGraph (LGraph_SGraph (Graph_LGraph G))) r ->
+                           dst (SGraph_PGraph (LGraph_SGraph (Graph_LGraph G))) (x, L) = l -> dst (SGraph_PGraph (LGraph_SGraph (Graph_LGraph G))) (x, R) = r ->
                            (ptto_node x v l r ⊗ (graph l G ⊗ graph r G)) =
                            graph l G ⊗ graphs (x :: l :: r :: nil)
-                                 (GraphBi.Graph_SpatialGraph G).
+                                 (LGraph_SGraph (Graph_LGraph G)).
   Proof.
     intros. simpl. rewrite ocon_emp. do 3 rewrite <- ocon_assoc.
     rewrite (ocon_comm (graph l G) (graph x G)).
@@ -279,18 +287,19 @@ Module GraphMark <: Mgraphmark.
     + apply precise_graph. apply RGF. left; intuition.
     + destruct H1 as [? [? [? [? [? ?]]]]]. destruct H2 as [? [? [? [? [? ?]]]]].
       rewrite (graph_graphs_eq_l G v x l r); auto. rewrite (graph_graphs_eq_l G1 v1 x l r); auto.
-      assert (forall (g: A), graph l g = graphs (l :: nil) (GraphBi.Graph_SpatialGraph g)) by (intros; simpl; rewrite ocon_emp; auto).
+      assert (forall (g: A), graph l g = graphs (l :: nil) (LGraph_SGraph (Graph_LGraph g))) by (intros; simpl; rewrite ocon_emp; auto).
       rewrite (H13 G). rewrite (H13 G1). apply subgraph_update; auto. apply RGF. apply RGF. 
       - intros. left. simpl in H14. destruct H14 as [? | [? | [? | [? | ?]]]]; [subst x0 ..|exfalso]; auto.
       - intros. left. simpl in H14. destruct H14 as [? | [? | [? | [? | ?]]]]; [subst x0 ..|exfalso]; auto.
   Qed.
 
   Lemma graph_graphs_eq_r:
-    forall (G: A) v x l r, vlabel G x = v -> vvalid G x -> vvalid G l -> vvalid G r ->
-                           dst G (x, L) = l -> dst G (x, R) = r ->
+    forall (G: A) v x l r, vlabel (Graph_LGraph G) x = v -> vvalid (SGraph_PGraph (LGraph_SGraph (Graph_LGraph G))) x ->
+                           vvalid (SGraph_PGraph (LGraph_SGraph (Graph_LGraph G))) l -> vvalid (SGraph_PGraph (LGraph_SGraph (Graph_LGraph G))) r ->
+                           dst (SGraph_PGraph (LGraph_SGraph (Graph_LGraph G))) (x, L) = l -> dst (SGraph_PGraph (LGraph_SGraph (Graph_LGraph G))) (x, R) = r ->
                            (ptto_node x v l r ⊗ (graph l G ⊗ graph r G)) =
                            graph r G ⊗ graphs (x :: l :: r :: nil)
-                                 (GraphBi.Graph_SpatialGraph G).
+                                 (LGraph_SGraph (Graph_LGraph G)).
   Proof.
     intros. simpl. rewrite ocon_emp. do 3 rewrite <- ocon_assoc.
     rewrite (ocon_comm (graph r G) (graph x G)).
@@ -309,7 +318,7 @@ Module GraphMark <: Mgraphmark.
     + apply (bi_graph_precise_left _ x); auto.
     + apply (bi_graph_precise_right _ x); auto.
   Qed.
-  
+
   Lemma lem_subgraphupdate_r : forall G v G1 x v1 l r, valid (imp (and (star (graph r G1) (mwand (graph r G) (union (ptto_node x v l r) (union (graph l G) (graph r G))))) (and (subset_reach G r G1) (and (eq_notreach G r G1) (and (lookup G x v l r) (lookup G1 x v1 l r))))) (union (ptto_node x v1 l r) (union (graph l G1) (graph r G1)))).
   Proof.
     intros. unfold valid, imp, and, star, mwand, union, subset_reach, eq_notreach, lookup.
@@ -317,7 +326,7 @@ Module GraphMark <: Mgraphmark.
     + apply precise_graph. apply RGF. left; intuition.
     + destruct H1 as [? [? [? [? [? ?]]]]]. destruct H2 as [? [? [? [? [? ?]]]]].
       rewrite (graph_graphs_eq_r G v x l r); auto. rewrite (graph_graphs_eq_r G1 v1 x l r); auto.
-      assert (forall (g: A), graph r g = graphs (r :: nil) (GraphBi.Graph_SpatialGraph g)) by (intros; simpl; rewrite ocon_emp; auto).
+      assert (forall (g: A), graph r g = graphs (r :: nil) (LGraph_SGraph (Graph_LGraph g))) by (intros; simpl; rewrite ocon_emp; auto).
       rewrite (H13 G). rewrite (H13 G1). apply subgraph_update; auto. apply RGF. apply RGF. 
       - intros. left. simpl in H14. destruct H14 as [? | [? | [? | [? | ?]]]]; [subst x0 ..|exfalso]; auto.
       - intros. left. simpl in H14. destruct H14 as [? | [? | [? | [? | ?]]]]; [subst x0 ..|exfalso]; auto.
@@ -330,16 +339,16 @@ Module GraphMark <: Mgraphmark.
     + unfold ptto_node. apply log_normalize.mapsto_precise.
     + destruct H as [? [? [? [? [? ?]]]]]. rewrite <- ocon_assoc. rewrite <- (lookup_graph_unfold G x v l r); auto.
       destruct H0 as [Hn [Hi ?]]. rewrite <- ocon_assoc.
-      assert (vgamma (GraphBi.Graph_SpatialGraph G) x = (v, l, r)). {
-        simpl. unfold gamma. f_equal; [f_equal |]; auto.
+      assert (vgamma (LGraph_SGraph (Graph_LGraph G)) x = (v, l, r)). {
+        simpl. f_equal; [f_equal |]; auto.
       } pose proof (Graph_gen_update_spatial_spec  G x v v1 l r Hi Hn H1 H6).
       pose proof (Graph_gen_update_vgamma G x v1 l r Hi Hn). rewrite H0 in H8.
-      simpl in H8. unfold gamma in H8. rewrite <- (lookup_graph_unfold G1 x v1 l r);
+      simpl in H8. rewrite <- (lookup_graph_unfold G1 x v1 l r);
         [| inversion H8 |rewrite <- H0; simpl; unfold graph_gen.change_vvalid ..|inversion H8|inversion H8]; auto.
       pose proof (graph_vi_eq _ _ x H7). rewrite H0 in H9. unfold graph at 2.
       unfold node in H9 at 1. rewrite H9. apply graph_ramify_aux0; auto. apply RGF.
   Qed.
-  
+
   Lemma axiom_1 : forall v G1 G2 G G3 x l r, valid (imp (and (lookup G x v l r) (and (mark G r G1) (and (neq v true) (and (mark G2 l G3) (update G1 x true l r G2))))) (and (mark G x G3) (lookup G3 x true l r))).
   Proof.
   Admitted.
